theories/RTL/SimRules.v
@@ -1,14 +1,13 @@
-From RSL Require Import Prelude RLogic.
+From RSL Require Import Prelude.
 
 From Coinduction Require Import all.
-
-From RSL Require Import Simulations.FreeSim.
 
 From RSL Require Import RTL.RTL.
 From RSL Require Import RTL.Semantics.
 From RSL Require Import RTL.Notations.
 
-From iris.proofmode Require Import proofmode.
+From RSL Require Import Simulations.FreeSim.
+From RSL Require Import Simulations.FreeSimRules.
 
 Import RTLNotations.
 
@@ -23,16 +22,13 @@ Section RulesDef.
 
   Definition sim C st j i ss (Q: post) : rlogic :=
     let Φ : value Λₜ -> value Λₛ -> Prop :=
-      fun '(vₜ, mₜ) '(vₛ, mₛ) => Q vₜ vₛ mₜ mₛ
+      fun '(vt, mt) '(vs, ms) => (Q vt vs) mt ms
     in
-    fun mₜ mₛ =>
-      fsim_lfp C Φ
-        j ([], st, mₜ)
-        i ([], ss, mₛ).
+    fun mt ms => fsim_lfp C Φ ([], st, mt) j i ([], ss, ms).
 
   Definition hoare C P st j i ss Q : rlogic :=
     (□ ∀ Φ, P -∗
-             (∀ vₜ vₛ, Q vₜ vₛ -∗ Φ vₜ vₛ) -∗
+             (∀ vt vs, Q vt vs -∗ Φ vt vs) -∗
              sim C st j i ss Φ)%I.
 
   Notation
@@ -45,150 +41,81 @@ Section RulesDef.
     (hoare C P%I st j i ss Q%I)
       (at level 0, no associativity).
 
-  (* Lemma both_ret C ρₜ ρₛ fₜ pcₜ j i fₛ pcₛ Q : *)
-  (*   ∀ rₜ vₜ rₛ vₛ, *)
-  (*   fₜ@pcₜ is <<{ ret rₜ }>> -> *)
-  (*   fₛ@pcₛ is <<{ ret rₛ }>> -> *)
-  (*   ρₜ @ rₜ ⇒ vₜ -> *)
-  (*   ρₛ @ rₛ ⇒ vₛ -> *)
-  (*   Q vₜ vₛ ⊢ [C] State fₜ pcₜ ρₜ <{j, i}= State fₛ pcₛ ρₛ {{ Q }}. *)
-  (* Proof using Type. *)
-  (*   intros rt vt rs vs Hpct Hpcs Ht Hs. *)
-  (*   intros mtQ msQ HQ. *)
-
-  (*   eapply FSourceSteps with (i' := 0). *)
-  (*   { eapply exec_Iret; eassumption. } *)
-
-  (*   eapply FTargetSteps. *)
-  (*   { eexists; eapply exec_Iret; eassumption. } *)
-
-  (*   intros t' Hstep. inv Hstep. exists 0. *)
-
-  (*   eapply FRelated. *)
-
-  (*   do 2 eexists; repeat split. simpl. *)
-  (*   simregs. assumption. *)
-  (* Qed. *)
-
-  Lemma frame C P1 P2 st j i ss Q :
-    [C] {{ P1 }} st <{j, i}= ss {{ fun vₜ vₛ => Q vₜ vₛ }}
-    ⊢
-    [C] {{ P1 ∗ P2 }} st <{j, i}= ss {{ fun vₜ vₛ => Q vₜ vₛ ∗ P2 }}.
+  Lemma both_ret C ρₜ ρₛ fₜ pcₜ j i fₛ pcₛ Q :
+    ∀ rₜ vₜ rₛ vₛ,
+    fₜ@pcₜ is <<{ ret rₜ }>> ->
+    fₛ@pcₛ is <<{ ret rₛ }>> ->
+    ρₜ @ rₜ ⇒ vₜ ->
+    ρₛ @ rₛ ⇒ vₛ ->
+    Q vₜ vₛ ⊢ [C] State fₜ pcₜ ρₜ <{j, i}= State fₛ pcₛ ρₛ {{ Q }}.
   Proof using Type.
-    iIntros "#H !> %Φ [HP1 HP2] Hpost".
-    iApply ("H" with "HP1").
-    iIntros "%vt %vs HQ".
-    iApply "Hpost".
-    iFrame.
+    intros rt vt rs vs Hpct Hpcs Ht Hs.
+    repeat unseal.
+    intros mtQ msQ HQ.
+
+    eapply FSourceSteps with (i' := 0).
+    { eapply exec_Iret; eassumption. }
+
+    eapply FTargetSteps.
+    { eexists; eapply exec_Iret; eassumption. }
+
+    intros t' Hstep. inv Hstep. exists 0.
+
+    eapply FRelated.
+
+    do 2 eexists; repeat split. simpl.
+    simregs. assumption.
   Qed.
 
-  Lemma consequence C P P' st j i ss Q Q' :
-    (P ⊢ P') ->
-    (∀ vₜ vₛ, Q' vₜ vₛ ⊢ Q vₜ vₛ) ->
-    [C] {{ P' }} st <{j, i}= ss {{ Q' }}
-    ⊢ [C] {{ P }} st <{j, i}= ss {{ Q }}.
+  Local Definition coind_inv
+    (Inv: (val → val → rlogic) -> pcstate -> pcstate -> rlogic)
+    (ϕ: value Λₜ → value Λₛ → Prop)
+    (t: state Λₜ) (j i: nat) (s: state Λₛ) : Prop :=
+    ∃ mt st ms ss,
+      t = ([], st, mt) ∧
+      s = ([], ss, ms) ∧
+      Inv (fun vt vs mt ms => ϕ (vt, mt) (vs, ms)) st ss mt ms.
+
+  Lemma coind Inv st j i ss Q :
+    ⊢ □ (∀ R st i j ss,
+           □ (∀ st j' i' ss,
+                ⌜i < i'⌟ -∗
+                ⌜j < j'⌟ -∗
+                Inv Q st ss -∗
+                [R] st <{j', i'}= ss {{ Q }}) -∗
+        Inv Q st ss -∗
+        [R] st <{j, i}= ss {{ Q }}
+      ) -∗
+      Inv Q st ss -∗
+      [fsim] st <{j, i}= ss {{ Q }}.
   Proof using Type.
-    iIntros (HP HQ) "#H !> %Φ Hpre Hpost".
-    iApply ("H" with "[Hpre]").
-    - iApply (HP). iAssumption.
-    - iIntros (vₜ vₛ) "HQ'".
-      iApply "Hpost". iApply (HQ). iAssumption.
+    unfold sim; unseal.
+    intros ? ? [-> ->] ? ? _ _ [[-> ->] RIH].
+    intros mtInv msInv _ _ Hinv.
+    eapply (coind_strong_open nat nat Pₜ Pₛ _ (coind_inv Inv)).
+    {
+      clear Hinv st ss i j mtInv msInv.
+      intros R ? j i ? CIH (mt & st & ms & ss & -> & -> & Hinv).
+      rewrite <- (map_empty_union mt).
+      rewrite <- (map_empty_union ms).
+      rewrite <- (map_empty_union ∅).
+      eapply RIH; auto; try solve_map_disjoint.
+      split. { easy. }
+      intros ? ? [-> ->] st' j' i' ss'.
+      intros ? ? _ _ [[-> ->] Hi].
+      intros ? ? _ _ [[-> ->] Hj].
+      intros mtInv msInv _ _ Hinv'.
+      apply CIH; auto.
+      exists mtInv, st', msInv, ss'.
+      repeat split.
+      - now rewrite !(map_empty_union _).
+      - now rewrite !(map_empty_union _).
+      - assumption.
+    }
+    exists mtInv, st, msInv, ss.
+    repeat split.
+    - now rewrite !(map_empty_union _).
+    - now rewrite !(map_empty_union _).
+    - assumption.
   Qed.
-
-  (* Local Lemma rewrite_hoare C P st j i ss Q : *)
-  (*   ( *)
-  (*     ∀ (Ψ: value Λₜ → value Λₛ → Prop) (mtP msP mtQ msQ : memory), *)
-  (*       ∀ Φ, *)
-  (*       (∀ vₜ vₛ mₜ mₛ, Φ vₜ vₛ mₜ mₛ <-> Ψ (vₜ, mₜ) (vₛ, mₛ)) ∧ *)
-  (*       mtP ##ₘ mtQ ∧ *)
-  (*       msP ##ₘ msQ ∧ *)
-  (*       P mtP msP ∧ *)
-  (*       (∀ (vₜ vₛ : val) (mt ms : memory), *)
-  (*          mt ##ₘ mtQ -> *)
-  (*          ms ##ₘ msQ -> *)
-  (*          Q vₜ vₛ mt ms -> *)
-  (*          Φ vₜ vₛ (mt ∪ mtQ) (ms ∪ msQ) *)
-  (*       ) -> *)
-  (*       fsim_lfp C (fun '(vₜ, mₜ) '(vₛ, mₛ) => Φ vₜ vₛ mₜ mₛ) *)
-  (*         j ([], st, mtQ ∪ mtP) *)
-  (*         i ([], ss, msQ ∪ msP) *)
-  (*   ) ⊣⊢ *)
-  (*   [C] {{ P }} st <{j, i}= ss {{ Q }}. *)
-  (* Proof using Type. *)
-  (*   split; intros H. *)
-  (*   - intros ? ? Hemp Ψ mtPre msPre ? ? Hpre mtPost msPost ? ? Hpost. *)
-  (*     destruct Hemp as (-> & ->). *)
-  (*     decompose_map_disjoint. *)
-  (*     unfold memory in *. *)
-  (*     rewrite !(map_union_empty _). *)
-  (*     apply H with (Ψ := fun '(vₜ, mₜ) '(vₛ, mₛ) => Ψ vₜ vₛ mₜ mₛ). *)
-  (*     repeat split; easy. *)
-  (*   - intros Ψ mtP msP mtQ msQ Φ (HΦ & Ht & Hs & Hpre & Hpost). *)
-  (*     rewrite <- (map_union_empty mtP). *)
-  (*     rewrite <- (map_union_empty msP). *)
-  (*     apply H. *)
-  (*     + now split. *)
-  (*     + solve_map_disjoint. *)
-  (*     + solve_map_disjoint. *)
-  (*     + assumption. *)
-  (*     + solve_map_disjoint. *)
-  (*     + solve_map_disjoint. *)
-  (*     + intros vₜ vₛ mt ms. *)
-  (*       apply Hpost. *)
-  (* Qed. *)
-
-  (* Lemma coind ρₜ ρₛ Inv fₜ pcₜ j i fₛ pcₛ Q : *)
-  (*   (∀ R ρₜ ρₛ, *)
-  (*      (∀ ρₜ ρₛ j' i', *)
-  (*         i < i' -> *)
-  (*         j < j' -> *)
-  (*         [R] (ρₜ, ρₛ) ⊢ {{ Inv ρₜ ρₛ }} fₜ @ pcₜ <{j', i'}= fₛ @ pcₛ {{ Q }}) -> *)
-  (*      [R] (ρₜ, ρₛ) ⊢ {{ Inv ρₜ ρₛ }} fₜ @ pcₜ <{j, i}= fₛ @ pcₛ {{ Q }} *)
-  (*   ) -> *)
-  (*   [fsim] (ρₜ, ρₛ) ⊢ {{ Inv ρₜ ρₛ }} fₜ @ pcₜ <{j, i}= fₛ @ pcₛ {{ Q }}. *)
-  (* Proof using Type. *)
-  (*   intros RIH. *)
-  (*   rewrite <- rewrite_hoare. *)
-  (*   intros Ψ mtP msP mtQ msQ Φ H. *)
-  (*   apply fsim_unroll. *)
-  (*   revert ρₜ ρₛ Ψ mtP msP mtQ msQ Φ H. *)
-  (*   coinduction C CIH. *)
-  (*   intros ρₜ ρₛ Ψ mtP msP mtQ msQ Φ (HΦ & Ht & Hs & Hpre & Hpost). *)
-  (*   rewrite <- (map_union_empty mtP). *)
-  (*   rewrite <- (map_union_empty msP). *)
-  (*   apply RIH. *)
-  (*   - intros ρₜ' ρₛ' j' i' Hi Hj. *)
-  (*     rewrite <- rewrite_hoare. *)
-  (*     repeat intro. *)
-  (*     eapply FProgress. *)
-  (*     { eassumption. } *)
-  (*     { eassumption. } *)
-  (*     eapply CIH. eassumption. *)
-  (*   - now split. *)
-  (*   - solve_map_disjoint. *)
-  (*   - solve_map_disjoint. *)
-  (*   - assumption. *)
-  (*   - solve_map_disjoint. *)
-  (*   - solve_map_disjoint. *)
-  (*   - intros vₜ vₛ mt ms. apply Hpost. *)
-  (* Qed. *)
-
-  (* Lemma fsim_mono ρₜ ρₛ P fₜ pcₜ j i fₛ pcₛ Q : *)
-  (*   ∀ j' i', *)
-  (*   (j' <= j)%nat -> *)
-  (*   (i' <= i)%nat -> *)
-  (*   [fsim] (ρₜ, ρₛ) ⊢ {{ P }} fₜ @ pcₜ <{j', i'}= fₛ @ pcₛ {{ Q }} -> *)
-  (*   [fsim] (ρₜ, ρₛ) ⊢ {{ P }} fₜ @ pcₜ <{j, i}= fₛ @ pcₛ {{ Q }}. *)
-  (* Proof using Type. *)
-  (*   intros i' j' Hi Hj H. *)
-  (*   intros ? ? Hemp Ψ mtPre msPre ? ? Hpre mtPost msPost ? ? Hpost. *)
-  (*   apply (gfp_fp fsim_lfp). *)
-  (*   eapply idx_mono. *)
-  (*   - apply (gfp_chain (chain_gfp fsim_lfp)). *)
-  (*     apply (gfp_fp fsim_lfp). *)
-  (*     now apply H. *)
-  (*   - unfold "⊑". simpl. lia. *)
-  (*   - unfold "⊑". simpl. lia. *)
-  (* Qed. *)
-
 End RulesDef.
