theories/RTL/SourceRules.v
@@ -1,6 +1,4 @@
-From RSL Require Import RelLogic Prelude.
-
-From Coinduction Require Import all.
+From RSL Require Import Prelude.
 
 From RSL Require Import Simulations.FreeSim.
 From RSL Require Import Simulations.FreeSimRules.
@@ -22,112 +20,115 @@ Section SourceRulesDef.
   Abbreviation fsim := (fsim WfNat WfNat Pₜ Pₛ).
 
   Notation
-    "'[' C ']' ρ '⊢' ft '@' pct  '<{' j ',' i '}=' fs '@' pcs '{{' Q '}}'" :=
-    (sim Pₜ Pₛ C ρ ft pct j i fs pcs Q%rlogic)
-      (at level 0, ft at level 0, fs at level 0, no associativity).
+    "'[' C ']' st '<{' j ',' i '}=' ss '{{' Q '}}'" :=
+    (sim Pₜ Pₛ C st j i ss Q%I)
+      (at level 0, no associativity).
 
-  Notation
-    "'[' C ']' ρ '⊢' '{{' P '}}' ft '@' pct  '<{' j ',' i '}=' fs '@' pcs '{{' Q '}}'" :=
-    (hoare Pₜ Pₛ C ρ P%rlogic ft pct j i fs pcs Q%rlogic)
-      (at level 0, ft at level 0, fs at level 0, no associativity).
-
-  Lemma source_nop C ρₜ ρₛ P fₜ pcₜ j i fₛ pcₛ Q :
+  Lemma source_nop C st j i fₛ pcₛ ρₛ Q :
     ∀ pc,
     fₛ@pcₛ is <<{ nop -> pc }>> ->
-    [C] (ρₜ, ρₛ) ⊢ {{ P }} fₜ @ pcₜ <{j, 1+i}= fₛ @ pc {{ Q }} ->
-    [C] (ρₜ, ρₛ) ⊢ {{ P }} fₜ @ pcₜ <{j, i}= fₛ @ pcₛ {{ Q }}.
+    ⊢ [C] st <{j, 1+i}= State fₛ pc ρₛ {{ Q }} -∗
+      [C] st <{j, i}= State fₛ pcₛ ρₛ {{ Q }}.
   Proof using Type.
-    intros pc Hpc H.
-    intros ? ? Hemp Ψ mtPre msPre ? ? Hpre mtPost msPost ? ? Hpost.
+    intros pc Hpc.
+    unseal. intros ? ? [-> ->] mt ms _ _ H.
+    rewrite !(map_empty_union _).
 
     eapply FSourceSteps.
     - econstructor; eassumption.
-    - now apply H.
+    - apply H.
   Qed.
 
-  Lemma source_op C ρₜ ρₛ P fₜ pcₜ j i fₛ pcₛ Q :
+  Lemma source_op C st j i fₛ pcₛ ρₛ Q :
     ∀ pc dst op regs args,
     fₛ@pcₛ is <<{ dst := @op regs -> pc }>> ->
     ρₛ @ regs ⇒ args ->
-    (∀ v, eval_op op args = Some v ->
-     [C] (ρₜ, ⟦dst ⇐ v⟧ρₛ) ⊢ {{ P }} fₜ @ pcₜ <{j, 1+i}= fₛ @ pc {{ Q }}) ->
-    [C] (ρₜ, ρₛ) ⊢ {{ P }} fₜ @ pcₜ <{j, i}= fₛ @ pcₛ {{ Q }}.
+    ⊢ (∀ v, ⌜eval_op op args = Some v⌟ -∗
+            [C] st <{j, 1+i}= State fₛ pc (⟦dst ⇐ v⟧ρₛ) {{ Q }}) -∗
+      [C] st <{j, i}= State fₛ pcₛ ρₛ {{ Q }}.
   Proof using Type.
-    intros pc dst op regs args Hpc Hargs H.
-    intros ? ? Hemp Ψ mtPre msPre ? ? Hpre mtPost msPost ? ? Hpost.
+    intros pc dst op regs args Hpc Hargs.
+    unseal. intros ? ? [-> ->] mt ms _ _ H.
 
     destruct (eval_op op args) as [v|] eqn:Hv.
     - eapply FSourceSteps.
       + econstructor; eassumption || reflexivity.
-      + now eapply H.
+      + rewrite <- (map_union_comm mt) by solve_map_disjoint.
+        rewrite <- (map_union_comm ms) by solve_map_disjoint.
+        eapply H; auto; solve_map_disjoint.
     - apply FSourceStuck.
-      split.
-      { reflexivity. }
+      split. { reflexivity. }
       intros Hprog. apply can_progress_must_step in Hprog.
       destruct Hprog as [? Hprog].
       inv Hprog. simregs.
   Qed.
 
-  Lemma source_load C ρₜ ρₛ P fₜ pcₜ j i fₛ pcₛ Q :
+  Lemma source_load C st j i fₛ pcₛ ρₛ Q :
     ∀ pc dst src addr v,
     fₛ@pcₛ is <<{ dst := !src -> pc }>> ->
     ρₛ @ src ⇒ addr ->
-    [C] (ρₜ, ⟦dst ⇐ v⟧ρₛ) ⊢ {{ addr →ₛ v ∗ P }} fₜ @ pcₜ <{j, 1+i}= fₛ @ pc {{ Q }} ->
-    [C] (ρₜ, ρₛ) ⊢ {{ addr →ₛ v ∗ P }} fₜ @ pcₜ <{j, i}= fₛ @ pcₛ {{ Q }}.
+    ⊢ addr →ₛ v -∗
+      (addr →ₛ v -∗
+       [C] st <{j, 1+i}= State fₛ pc (⟦dst ⇐ v⟧ρₛ) {{ Q }}) -∗
+      [C] st <{j, i}= State fₛ pcₛ ρₛ {{ Q }}.
   Proof using Type.
-    intros pc dst src addr v Hpc Haddr H.
-    intros ? ? Hemp Ψ mtPre msPre ? ? Hpre mtPost msPost ? ? Hpost.
-
-    destruct Hpre as (mtAddr & msAddr & mtP & msP & ? & ? & ? & ? & Hm & HP).
-    destruct Hm as (Ht & (l & Hl & Hs)).
+    intros pc dst src addr v Hpc Haddr.
+    unfold sim; unseal.
+    unseal. intros ? ? [-> ->] mt ms _ _ [-> (l & Hloc & ->)].
+    rewrite !(map_empty_union _). intros mt ms ? ? H.
 
     eapply FSourceSteps.
     - eapply exec_Iload with (v := v); try eassumption.
-      + subst. now simget.
+      + subst. simget.
       + reflexivity.
-    - apply H; auto.
-      eexists mtAddr, msAddr, mtP, msP.
-      repeat split; auto.
-      eexists. split; eassumption.
+    - rewrite <- (map_union_comm mt) by solve_map_disjoint.
+      rewrite <- (map_union_comm ms) by solve_map_disjoint.
+
+      eapply H; auto; try solve_map_disjoint.
+      repeat split.
+      eexists. split; eassumption || reflexivity.
   Qed.
 
-  Lemma source_store C ρₜ ρₛ P fₜ pcₜ j i fₛ pcₛ Q :
+  Lemma source_store C st j i fₛ pcₛ ρₛ Q :
     ∀ pc dst src addr v old,
     fₛ@pcₛ is <<{ !dst := src -> pc }>> ->
     ρₛ @ dst ⇒ addr ->
     ρₛ @ src ⇒ v ->
-    [C] (ρₜ, ρₛ) ⊢ {{ addr →ₛ v ∗ P }} fₜ @ pcₜ <{j, 1+i}= fₛ @ pc {{ Q }} ->
-    [C] (ρₜ, ρₛ) ⊢ {{ addr →ₛ old ∗ P }} fₜ @ pcₜ <{j, i}= fₛ @ pcₛ {{ Q }}.
+    ⊢
+      addr →ₛ old -∗
+      (addr →ₛ v -∗ [C] st <{j, 1+i}= State fₛ pc ρₛ {{ Q }}) -∗
+      [C] st <{j, i}= State fₛ pcₛ ρₛ {{ Q }}.
   Proof using Type.
-    intros pc dst src addr v old Hpc Haddr Hv H.
-    intros ? ? Hemp Ψ mtPre msPre ? ? Hpre mtPost msPost ? ? Hpost.
-
-    destruct Hpre as (mtAddr & msAddr & mtP & msP & ? & ? & ? & ? & Hm & HP).
-    destruct Hm as (Ht & (l & Hl & Hs)).
+    intros pc dst src addr v old Hpc Haddr Hv.
+    unseal. intros ? ? [-> ->] mt ms _ _ [-> (l & Hloc & ->)].
+    rewrite !(map_empty_union _). intros mtP msP ? ? H.
 
     eapply FSourceSteps.
     - eapply exec_Istore; try eassumption.
-      subst. erewrite (set_at_some  _ _ _ _ _ Hl) by now simget.
-      rewrite !alter_union_right by solve_map_disjoint.
-      rewrite !alter_union_left by solve_map_disjoint.
+      subst.
+      erewrite (set_at_some  _ _ _ _ _ Hloc) by simget.
+      erewrite alter_union_left by solve_map_disjoint.
       rewrite !alter_singleton.
       reflexivity.
-    - subst. apply H; try solve_map_disjoint.
-      eexists ∅, _, mtP, msP. repeat split; eauto.
-      + solve_map_disjoint.
-      + exists l. now split.
+    - subst.
+      rewrite <- (map_union_comm mtP) by solve_map_disjoint.
+      rewrite <- (map_union_comm msP) by solve_map_disjoint.
+      eapply H; auto; try solve_map_disjoint.
+      repeat split.
+      eexists. split; eassumption || reflexivity.
   Qed.
 
-  Lemma source_if C ρₜ ρₛ P fₜ pcₜ j i fₛ pcₛ Q :
+  Lemma source_if C st j i fₛ pcₛ ρₛ Q :
     ∀ pc_true pc_false reg v pc,
     fₛ@pcₛ is <<{ if reg then goto pc_true else goto pc_false }>> ->
     ρₛ @ reg ⇒ v ->
     (if (v =? 0)%Z then pc_true else pc_false) = pc ->
-    [C] (ρₜ, ρₛ) ⊢ {{ P }} fₜ @ pcₜ <{j, 1+i}= fₛ @ pc {{ Q }} ->
-    [C] (ρₜ, ρₛ) ⊢ {{ P }} fₜ @ pcₜ <{j, i}= fₛ @ pcₛ {{ Q }}.
+    ⊢ [C] st <{j, 1+i}= State fₛ pc ρₛ {{ Q }} -∗
+      [C] st <{j, i}= State fₛ pcₛ ρₛ {{ Q }}.
   Proof using Type.
-    intros pc_true pc_false reg v pc Hpc Hv Hnext_pc H.
-    intros ? ? Hemp Ψ mtPre msPre ? ? Hpre mtPost msPost ? ? Hpost.
+    intros pc_true pc_false reg v pc Hpc Hv Hnext_pc.
+    unseal. intros ? ? [-> ->] mt ms _ _ H.
+    rewrite !(map_empty_union _).
 
     eapply FSourceSteps.
     - econstructor; eassumption || reflexivity.
